# Other

### Substitution & Elimination

**Elimination**

$$\begin{cases} 3x + 4y = 7 \\ 2x + 3y = 5 \end{cases}$$

Multiply the top by $$2$$ and the bottom by $$-3$$:

$$\begin{cases} 6x + 8y = 14 \\ -6x - 9y = -15 \end{cases}$$

$$-y = -1 \implies y = 1$$

$$2x + 3(1) = 5 \implies 2x = 2 \implies x = 1$$

$$(1, 1)$$

***

**Substitution**

$$\begin{cases} 2x - 3y = -2 \\ 4x + y = 24 \end{cases}$$

Isolate $$y$$ in the second equation: $$y = 24 - 4x$$

Substitute into the first: $$2x - 3(24 - 4x) = -2$$

$$2x - 72 + 12x = -2$$

$$14x = 70 \implies x = 5$$

Substitute: $$y = 24 - 4(5) \implies y = 4$$

$$(5, 4)$$

### General Transformations

**General transformation** is used to describe how a "parent" graph is moved, stretched, or flipped on a coordinate plane.

$$f(x) = a \cdot b^{x-h} + k$$

The **Vertical** Shift ($$k$$)

* The value of $$k$$ controls the Horizontal Asymptote (the invisible floor).
* If $$k$$ is positive ($$+3$$): The entire graph slides up 3 units. Your "floor" moves from $$y=0$$ to $$y=3$$.
* If $$k$$ is negative ($$-5$$): The entire graph slides down 5 units. Your "floor" is now at $$y=-5$$.

The **Horizontal** $$h$$ value sits in the exponent with $$x$$. This transformation moves the graph in the opposite direction of the sign you see.

* If you see $$(x - 3)$$: The graph moves Right 3 units.
* If you see $$(x + 2)$$: The graph moves Left 2 units.
* Why is it backward? To get the same output ($$y$$) as the original graph, you now have to use an $$x$$ value that is 3 units larger to "cancel out" the $$-3$$.

The **Vertical Stretch/Compression** $$a$$ value (the number in front) acts like you are grabbing the graph and pulling it taller or squishing it flatter.

* If $$|a| > 1$$: The graph gets "steep" faster (Vertical Stretch).
* If $$0 < |a| < 1$$: The graph looks flatter (Vertical Compression).
* If $$a$$ is negative ($$-a$$): The graph flips over the x-axis. Instead of exploding upward, it explodes downward.

$$f(x) = 2^{x-3} + 1$$:

1. Identify $$k$$: The asymptote is at $$y = 1$$. Draw a dashed line there first.
2. Identify $$h$$: The graph is moved Right 3.
3.  Find Y-Intercept: Plug in $$x = 0$$ to find exactly where it hits the y-axis.

    $$f(0) = 2^{0-3} + 1 = 2^{-3} + 1 = \frac{1}{8} + 1 = 1.125$$

### Inverse Functions

The $$-1$$ in $$f^{-1}(x)$$ is not an exponent. It doesn't mean $$\frac{1}{f(x)}$$. It is simply a special symbol used to label the inverse

Find the inverse of $$f(x) = 2x + 3$$

1.  Replace $$f(x)$$ with $$y$$

    $$y = 2x + 3$$
2.  Swap $$x$$ and $$y$$

    $$x = 2y + 3$$
3.  Solve for the new $$y$$

    $$x - 3 = 2y$$\
    $$\frac{x - 3}{2} = y$$
4.  Replace $$y$$ with $$f^{-1}(x)$$

    $$f^{-1}(x) = \frac{x - 3}{2}$$

### Function Composition

$$f(g(x))$$ is called a composite function

the output of $$g(x)$$ becomes the input for $$f(x)$$

### Trigonometry

### Conic Sections

$$(x-h)^2 + (y-k)^2 = r^2$$

every point $$(x, y)$$ that lies on the edge of a specific circle

$$(h, k)$$: These are the coordinates of the Center of the circle.

* $$h$$ is the x-coordinate (left/right).
* $$k$$ is the y-coordinate (up/down).

$$r$$: This is the Radius (the distance from the center to the edge).

* Note: In the equation, the radius is squared ($$r^2$$).

$$(x, y)$$: These represent any point on the boundary of the circle.

If a circle is centered at $$(0, 0)$$ with a radius of $$5$$:

* $$(x - 0)^2 + (y - 0)^2 = 5^2$$
* $$x^2 + y^2 = 25$$

### Probability and Statistics
